clean up Mirek's tutorial

TacticProgrammingGuide.lean
@@ -2,27 +2,27 @@ import Lean -- Lean's metaprogramming
 import Batteries
 import Qq -- convenient term building / matching
 
+namespace MetaProgrammingTutorial
+
 /-
-This tutorial is intended for people who have basic knowledge of
-Lean theorem prover, as well as some basic programming,
-and would be interested to know how to implement a custom tactic in Lean.
+This tutorial is intended for people who have basic knowledge of the Lean theorem prover,
+as well as some basic programming experience, and would be interested to know how to
+implement a custom tactic in Lean.
 
 Ideally open this file in VSCode to see how Lean reacts.
 
-After going through this tutorial, you should have a decent overview
-of what Lean metaprogramming is about, and be able to write some
-simple tactics.
+After going through this tutorial, you should have a decent overview of what
+Lean metaprogramming is about, and be able to write some simple tactics.
 
 # Beginner's Guide to Lean Tactic Programming
 
 Tactics are in principle arbitrary programs that opearate on the proof state.
-We can write such programs in place in the tactic proof, such as in
-the following example.
+We can write such programs in place in the tactic proof, such as in the following example.
 
 This example tactic doesn't do anything except logging "Hello world".
 Put your cursor at the blue-underlined run_tac to see the message.
 
-Do not bother by the type of Lean.logInfo too much so far,
+Do not bother with the type of `Lean.logInfo` too much so far,
 it is simply a logging / printing function.
 -/
 
@@ -43,35 +43,30 @@ Let us answer them.
 
 ## (1) How imperative programs work in Lean
 
-Lean is a pure functional language -- compared to
-imperative languages (C, Python, ...),
-its definitions cannot change, and its functions depend only on the arguments,
+Lean is a pure functional language - compared to imperative languages (C, Python, ...),
+its definitions cannot change, and its functions depend only on their arguments,
 and cannot have side effects.
 
 However, functional programming languages (such as Haskell) developed
 a way to write imperative style through
-* theory of monads
-* do syntax to hide most of monads from the user.
+* the theory of monads
+* "do notation" to hide most of monads from the user.
 
-We will keep the monad theory hidden, here we just say that a monad
-in general denotes an imperative program. There are several monads depending
-on what state they have access to. In the following example, we show
-two monads.
+We will keep the monad theory hidden, here we just say that a monad in general denotes
+an imperative program. There are several monads depending on what state they have access to.
+In the following example, we show two monads.
 
-Lean.Elab.Tactic.TacticM -- the top level tactic monad, has access to
-  all the data from the proofstate
-Lean.Meta.MetaM -- a monad that only has access to information about
-  metavariables (not important for now). This is a part of the entire
-  proofstate, so a TacticM can call a MetaM but not the other way around
-  (we would have to provide the TacticM all the extra data it needs)
+`Lean.Elab.Tactic.TacticM` - the top level tactic monad, has access to all the data
+  from the proofstate
+`Lean.Meta.MetaM` - a monad that only has access to information about metavariables
+  (not important for now). This is a part of the entire proofstate, so a `TacticM`
+  can call a `MetaM` but not the other way around (we would have to provide the
+  `TacticM` all the extra data it needs)
 
-We demostrate imperative programming in Lean
-by showing an example. So far, we are not using any API to access
-the proofstate (except logInfo), only showcase Lean as an imperative
-programming language.
+We will now demostrate imperative programming in Lean with some examples. So far,
+we are not using any API to access the proofstate (except `logInfo`), only showcasing
+Lean as an imperative programming language.
 -/
-
-namespace Chapter1Coding
 
 --         parameters     monad type   return value
 --             v               v         v
@@ -85,25 +80,24 @@ def myCode1 (n : Nat) : Lean.Meta.MetaM Nat := do
 --         parameters       monad type    no return value (like void in C)
 --             v                  v               v
 def myCode2 (n : Nat) : Lean.Elab.Tactic.TacticM Unit := do
-  Lean.logInfo m!"Calling Tactic1 ({n})"
+  Lean.logInfo m!"Calling myCode2 {n}"
 
 -- Array is basically the same thing as List with a different
 -- implementation (analogous to C++ vectors)
 def myCode3 : Lean.Elab.Tactic.TacticM (Array Nat) := do
-  Lean.logInfo "Calling Tactic2"
+  Lean.logInfo "Calling myCode3"
   myCode2 7
    -- lean variables are immutable but the do notation
    -- allows to break this using "let mut"
   let mut a : Array Nat := #[] -- "#" denotes it is an empty Array instead of empty List
-  for i in List.range 5 do
+  for i in [:5] do -- `[:5]` or `[0:5]` is short for `Std.Range.mk (start := 0) (stop := 5)`
     let res ← myCode1 i -- we use "←" to retrieve a value from a monad execution
-    a := a.push res -- an assignment without "let" only allowed for mutable variables
+    a := a.push res -- an assignment without "let" is only allowed for mutable variables
     -- Note: since we immediatelly replace a with (a.push i),
     --   Lean's inner optimization will avoid duplicating the array
     -- Note for imperative programmers:
-    --   "a.push res" alone cannot work, an external function cannot
-    --   change the value of "a", Lean is a pure functional language
-    --   after all
+    --   `a.push res` alone cannot work, an external function cannot change the value of "a".
+    --   Lean is a pure functional language after all
     Lean.logInfo m!"got: {res}"
   myCode2 15
   return a
@@ -117,34 +111,28 @@ example : True := by
     Lean.logInfo "Running some tactic programs 2!"
     let x ← myCode3
     -- Notice that it is possible to inline monad evaluation
-    -- inside an expression, using (← someTactic)
+    -- inside an expression, using `← someTactic`
     Lean.logInfo m!"result: {x} %% {← myCode1 5}"
   trivial
-
-end Chapter1Coding
 
 /-
 Of course, this is not exhaustive. Advanced topics include
 * What is the theory behind monads, how to use custom monads.
 * What are further programming-focused functions & datastructures in Lean,
-  such as Std.HashMap, foldM, IO monad, etc
-* different types of exceptions -- panic, throwError
+  such as `Std.HashMap`, `foldM`, the `IO` monad, etc
+* different types of exceptions -- `throwError`, `panic!`
 ...
 
 ## (2) What really is a proof state
 
-On the core level, a proof is a term, so called "proof term" that
-testifies the truth of the given proposition.
-When we are proving a theorem, at every moment, we have a partially
-built proof term with holes, so called metavariables.
-Once all metavariables are assigned, the proof is finished.
-Syntactically, metavariables start with a questionmark.
+On the core level, a proof is a term, a so called "proof term" that testifies the truth
+of the given proposition. When we are proving a theorem, at every moment, we have a partially
+built proof term with holes, so called metavariables. Once all metavariables are assigned,
+the proof is finished. Metavariables are the variables with a question mark before their name.
 
-As an example, we show a proof of "p → p ∧ True", and write
+As an example, we will show a proof of `p → p ∧ True`, and write
 the partially filled proof term in between.
 -/
-
-namespace Chapter2Datatypes
 
 theorem p_imp_p_true (p : Prop) : p → p ∧ True := by
   -- example : p → p ∧ True := ?_
@@ -157,29 +145,25 @@ theorem p_imp_p_true (p : Prop) : p → p ∧ True := by
   trivial
   -- example : p → p ∧ True := (fun h => And.intro h True.intro)
 
-end Chapter2Datatypes
-
 /-
 ## (3) What are the basic data structures around Lean metaprogramming
 
-* Expressions -- Lean.Expr, Qq
-* data in expressions: Lean.Name, Lean.MVarId, Lean.FVarId
-* printing: String, Format, MessageData
+* Expressions - `Lean.Expr`, `Qq`
+* data in expressions: `Lean.Name`, `Lean.MVarId`, `Lean.FVarId`
+* printing: `String`, `Format`, `MessageData`
 -/
 
-namespace Chapter3Datatypes
-
--- The basic data format is Expression -- ctrl-click
--- on Lean.Expr below to check its definition in the library.
+-- The data structure that is used to represent Lean exprssions is `Lean.Expr`.
+-- Due to the nature of dependent type theory, `Lean.Expr` is used to encode types, terms and proofs.
+-- Thus, `Lean.Expr` is also what is checked by the Lean kernel when checking proofs.
+-- ctrl-click on `Lean.Expr` below to see its definition in the library.
 #check Lean.Expr
--- Due to the nature of dependent type theory,
--- expressions are used for terms, propositions, types, and proofs.
 
--- Lean has a handy library Qq to build Expr with a convenient notation.
+-- Lean has a handy library Qq to help you build `Lean.Expr` terms with a convenient notation.
 open Qq
 
--- Q(...) is a type annotation of an expression, and
--- q(...) is
+-- `Q(...)` is a type annotation of an expression, and
+-- `q(...)` is an expression
 def t1 : Q(Prop) := q(True)
 def t2 : Q(Prop) := q(∀ p : Prop, p → p ∧ True)
 
@@ -188,73 +172,70 @@ def t2 : Q(Prop) := q(∀ p : Prop, p → p ∧ True)
 #eval t1
 #eval t2
 
--- The type in Qq is not explicitly Expr but it is definitionally equal to it,
--- and it is not forced to have a correct type. So think of Qq a bit as of
--- Python type annotations -- it can catch basic errors but it is not
--- forced at all.
+-- The type `Q(...)` is not explicitly `Lean.Expr` but it is definitionally equal to it,
+-- and it is not forced to have a correct type annotation. So you can think of Qq
+-- as of Python type annotations - it can catch basic errors but it is not forced at all.
 def t1e : Lean.Expr := t1
 def t1x : Q(Nat) := t1
 
 #check t1e
 #check t1x
 
--- Basically all metaprogramming types are in namespace Lean,
+-- Basically all metaprogramming API is in the namespace `Lean`
 -- repeating the prefix is getting annoying
 open Lean
 
--- Further important type used in Lean Metaprogramming is
-
--- Lean.Name
-def n1 : Name := `Nat.blah -- single backtick = arbitrary name
-def n2 : Name := ``t1e -- double backtick = resolve name
+-- Another important type in metaprogramming is `Lean.Name`
+def n1 : Name := `Nat.blah -- single backtick: arbitrary name
+def n2 : Name := ``t1e -- double backtick: resolved name (resolved in the currenct context)
 
 #print n1
 #print n2
 
--- The way Expr handles variables might seem messy at first -- there are
-#check Expr.bvar -- variable bound / quantified inside that Expr, represented with an index
+-- The way Expr handles variables might seem messy at first - there are
+#check Expr.bvar -- variable bound / quantified inside that `Expr`, represented with an index
 #check Expr.fvar -- named variable in the context
 #check Expr.mvar -- metavariable
 #check Expr.const -- a defined constant
 
--- Moreover, the username is never a unique identifier of a variable,
--- Lean wants to allow in principle multiple variables with the same name.
--- so free variables are identified by
+-- Moreover, user facing names of free variables and metavariables are not a unique
+-- identifier of a variable - Lean wants to allow multiple variables with the same name.
+-- So, free variables are identified by
 #check FVarId
+-- and metavariables are identified by
 #check MVarId
--- these datatypes hide a name inside too but that name (such as _uniq.13541)
+-- these datatypes hide a name inside too but that name (such as `_uniq.13541`)
 -- should never be ever exposed to the user.
 
 /-
-Showing / printing.
-Our basic printing function logInfo is a bit trickier, in normal
-programming languages, we are used to a print function that takes a
-String. However, in Lean, logInfo can show a term that allows
-mouse hover showing types, etc. In fact, there is
+### Showing / printing.
+Our basic printing function `logInfo` is a bit fancier that a you might expect.
+In normal programming languages, we are used to a print function that takes a `String`.
+However, in Lean, `logInfo` takes a `Lean.MessageData`. This means that it can show a term
+with mouse hover showing types and ctrl+click to go to definitions.
 -/
 #check MessageData -- interactive expression
-#check Format -- almost string (with) pretty-printing metadata)
 #check String -- standard list of characters
+#check Format -- string with information about how to line-wrap nicely
 
 -- Examine the print of the following logInfo.
 example : True := by
   run_tac
-    logInfo m!"Interactive MessageData: {t2}"
-    logInfo s!"String: {t2}"
+    logInfo m!"Interactive MessageData: t2 = {t2}"
+    logInfo s!"String: t2 = {t2}"
+    -- the function `repr` allows us to print the underlying data type.
+    -- it returns a `Format`.
+    logInfo f!"Format : repr t2 = {repr t2}"
   trivial
-
-end Chapter3Datatypes
 
 /-
 ## (4) Basic API to modify the proof state
 
 Let us write the code for the 4 tactics used in
 -/
-#check Chapter2Datatypes.p_imp_p_true
+#check p_imp_p_true
 example (p : Prop) : p → p ∧ True := by
   intro h; constructor; assumption; trivial
-
-namespace Chapter4TacticCode
 
 /-
 A lot of the functions / types are hidden in namespaces
@@ -264,7 +245,7 @@ A lot of the functions / types are hidden in namespaces
 so let's open them
 -/
 
-open Lean Meta Lean.Elab.Tactic Qq
+open Lean Meta Elab.Tactic Qq
 
 -- The easiest tactic to replace is "trivial"
 def runTrivial0 : TacticM Unit := do
@@ -272,7 +253,7 @@ def runTrivial0 : TacticM Unit := do
   let goal : MVarId ← getMainGoal
   -- and assign it to be True.intro
   goal.assign q(True.intro) -- !!! first attempt, not ideal
-  -- better to avoid low-level MVarId.assign, we will see why
+  -- better to avoid low-level `MVarId.assign`, we will see why
 
 example (p : Prop) : p → p ∧ True := by
   intro h; constructor; assumption
@@ -292,47 +273,63 @@ example (p : Prop) : p → p ∧ True := by -- !!!
   run_tac runTrivial0
 
 /-
-MVarId.assign happily closed the goal. Then we correctly
-closed the goal (?right : True), and at the very end,
-after Lean examined the entire proof term, we got
-a mysterious error that we cannot put together
-"@And.intro p True" and "True.intro"
-because it expects a proof of p.
+MVarId.assign happily closed the goal. Then we correctly closed the goal
+`?right : True`, and at the very end, after the Lean kernel checked
+the entire proof term, we got a mysterious error that we cannot apply
+`@And.intro p True` to `True.intro` because it expects a proof of `p`,
+and not a proof of `True`.
 
-Such errors are hard to decode, so it is better to ensure
-that we only set a mvar when we can.
-Fortunatelly, Batteries have
-a function that checks if something can be assigned.
+Such errors are hard to decode, so it is better to ensure that we only
+assign a metavariable if the assignment has the correct type.
+Fortunatelly, Batteries has a function that checks if something can be assigned.
+ctrl+click on it to see the implementation.
 -/
 #check MVarId.assignIfDefEq
 
--- correct version
-def runTrivial : TacticM Unit := do
+-- version throwing an error if the goal isn't `True`
+def runTrivial1 : TacticM Unit := do
   -- we retrieve the metavariable represesnting the current goal
   let goal : MVarId ← getMainGoal
   -- and assign it to be True.intro
   goal.assignIfDefEq q(True.intro)
 
--- now we got the correct error if we try to run runTrivial2
+-- now we get an error in the correct place if we try to run `runTrivial1`
 -- on the wrong goal
 example (p : Prop) : p → p ∧ True := by
   intro h; constructor
-  run_tac runTrivial -- error where it should be :-)
-  run_tac runTrivial
+  run_tac runTrivial1 -- error where it should be :-)
+  run_tac runTrivial1
 
 /-
-To implement assumption, we want to loop through
-all the assumptions, and try to use them.
-So we need
-* Access to the assumptions
-* Exception handling
+However, the error message "failed", is not very helpful.
+To improve this, we can catch that error, and provide our own, more useful error.
+We can catch errors using a `try ... catch _ => ...` block.
+And we can throw errors using `throwError`.
+-/
+def runTrivial : TacticM Unit := do
+  -- we retrieve the metavariable represesnting the current goal
+  let goal : MVarId ← getMainGoal
+  -- and assign it to be True.intro
+  try
+    goal.assignIfDefEq q(True.intro)
+  catch _ =>
+    let goalType ← goal.getType
+    throwError "tactic runTrivial1 failed, the goal has type `{goalType}` instead of `True`"
 
-How do we get the local context? In general contexts are
-assigned to metavariables but we can just use
-withMainContext.
-It stores the context assigned to the current goal
-in the monadic state,
-and then retrieve the context using getLCtx
+example (p : Prop) : p → p ∧ True := by
+  intro h; constructor
+  run_tac runTrivial -- now we get a useful error message here
+  run_tac runTrivial
+
+
+/-
+To implement `assumption`, we want to loop through all the assumptions,
+and try to use them one by one.
+The list of assumptions, which appears above the `⊢` in the infoview, is called
+the local context. How do we get the local context? In general each metavariable
+has its own local context, but we can just use `withMainContext`.
+This puts the local context of the current goal into the monadic context,
+and then we can retrieve the context using `getLCtx`
 
 First, we can just print the assumptions.
 -/
@@ -344,13 +341,8 @@ example (n : Nat) (hn : n > 5) : True := by
     withMainContext do
       let ctx ← getLCtx
       -- go through all local declarations
-      -- Note: the questionmark in decl? is just a part of the name
-      --   (good practice for Option type)
-      for (decl? : Option LocalDecl) in ctx.decls do
-        match decl? with
-        | some (decl : LocalDecl) =>
-          logInfo m!"{mkFVar decl.fvarId} : {decl.type}  -- {repr decl.kind}"
-        | none => pure ()
+      for (decl : LocalDecl) in ctx do
+        logInfo m!"{Expr.fvar decl.fvarId} : {decl.type}  -- {repr decl.kind}"
   trivial
 
 -- We have all the components, so let's implement the assumption tactic.
@@ -359,16 +351,13 @@ def runAssumption : TacticM Unit := -- we don't have to start with do here (but 
   withMainContext do -- but have to "do" it here
     let goal ← getMainGoal
     let ctx ← getLCtx
-    for (decl? : Option LocalDecl) in ctx.decls do
-      match decl? with
-      | some (decl : LocalDecl) =>
-        if decl.kind != .default then continue
-        try
-          goal.assignIfDefEq (mkFVar decl.fvarId)
-          return -- if succeeded, we are done
-        catch _ =>
-          pure () -- ignore the exception
-      | none => pure ()
+    for (decl : LocalDecl) in ctx do
+      if decl.kind != .default then continue
+      try
+        goal.assignIfDefEq (Expr.fvar decl.fvarId)
+        return -- if succeeded, we are done
+      catch _ =>
+        pure () -- ignore the exception
     throwError "Assumption not found"
 
 -- let's test
@@ -379,13 +368,12 @@ example (p : Prop) : p → p ∧ True := by
 
 /-
 The remaining two tactics require creating a new metavariable.
-A new metavariable is created using.
+A new metavariable is created using
 -/
 #check mkFreshExprMVar
 /-
-However a good practice is to make the goal variables
-"syntheticOpaque" -- then Lean knows that they are somewhat
-important, and doesn't unify them willy-nilly.
+However a good practice is to make the goal variables "syntheticOpaque" - then Lean
+knows that they are somewhat important, and doesn't unify them willy-nilly.
 
 One way is to use the following function
 -/
@@ -396,36 +384,33 @@ calls mkFreshExprMVar with a specific kind.
 -/
 
 /-
-In our runConstructor, we will decompose And.
+Now let us define `runConstructor`, in which we will decompose `And`.
 (we will not attempt general constructor)
-First, we just write the function that reads the type A ∧ B from the goal,
-and extracts the two type expressions A and B.
+First, we just write the function that reads the type `A ∧ B` from the goal,
+and extracts the two type expressions `A` and `B`.
 -/
 def extractAndGoals1 : TacticM (Expr × Expr) := do
-  let tgt ← getMainTarget -- equivalent to (← getGoal).getType
-  have quotedTgt : Q(Prop) := tgt -- change the apparent type
+  let tgt ← getMainTarget -- equivalent to `(← getGoal).getType`
+  have quotedTgt : Q(Prop) := tgt -- add a `Q(...)` annotation to `tgt`
   match quotedTgt with
   | ~q($p ∧ $q) => -- Qq match, must run in MetaM or higher
     return (p, q)
-  | _ => throwError m!"Goal {tgt} is not of the form (?_ ∧ ?_)"
+  | _ => throwError "Goal {tgt} is not of the form (?_ ∧ ?_)"
 
-/-
-Qq is handy but it is worth knowing how to do these
-things "manually"
--/
+-- Qq is handy but it is worth knowing how to do these things "manually"
 def extractAndGoals2 : TacticM (Expr × Expr) := do
   let tgt ← getMainTarget
   -- an alternative syntax to match ... with
   let (`And, #[p, q]) := tgt.getAppFnArgs
-    | throwError m!"Goal {tgt} is not of the form (?_ ∧ ?_)"
+    | throwError "Goal {tgt} is not of the form (?_ ∧ ?_)"
   return (p, q)
 
 -- let's check that our decomposition of "And" works.
 example (p q : Prop) (h : p ∧ q) : p ∧ q := by
   run_tac
-    let (a1,b1) ← extractAndGoals1
+    let (a1, b1) ← extractAndGoals1
     logInfo m!"Qq extraction: {a1} AND {b1}"
-    let (a2,b2) ← extractAndGoals2
+    let (a2, b2) ← extractAndGoals2
     logInfo m!"Expr extraction: {a1} AND {b1}"
   assumption
 
@@ -439,7 +424,7 @@ def runConstructor : TacticM Unit := do
     let ((a : Q(Prop)), (b : Q(Prop))) ← extractAndGoals1
     let left : Q($a) ← mkFreshExprMVar a (userName := `left) -- build new metavariables
     let right : Q($b) ← mkFreshExprMVar b (userName := `right)
-    goal.assign q(And.intro $left $right) -- can we be brave here with .assign? :-)
+    goal.assign q(And.intro $left $right) -- can we be brave here with `.assign`? :-)
     -- the list of active goals is not maintained automatically,
     -- we need to tell the proof state that we created two new goals
     replaceMainGoal [left.mvarId!, right.mvarId!]
@@ -451,18 +436,19 @@ example (p : Prop) : p → p ∧ True := by
   run_tac runAssumption
   run_tac runTrivial
 
-def runIntro (name : Name) : TacticM Unit := do
+def runIntro (name : Name) : TacticM Unit :=
   withMainContext do
     let goal ← getMainGoal
     let lctx ← getLCtx
     let .forallE _ type body c ← goal.getType
-      | throwError "Goal not of the form of an implication or quantification"
+      | throwError "Goal not of the form `_ → _` or `∀ _, _`"
     let fvarId : FVarId ← mkFreshFVarId -- allocate new variable
     let lctx' := lctx.mkLocalDecl fvarId name type c -- put into a new context
-    let fvar : Expr := mkFVar fvarId
+    let fvar : Expr := .fvar fvarId
     let body := body.instantiate1 fvar -- convert bvar to fvar
     withLCtx' lctx' do
-      -- mkFreshExprMVar uses the current monadic context to
+      -- `mkFreshExprMVar` uses the monadic context to determine the
+      -- local context of the new metavariable
       let newMVar ← mkFreshExprMVar body (kind := .syntheticOpaque)
       let newVal ← mkLambdaFVars #[fvar] newMVar
       goal.assign newVal
@@ -492,11 +478,11 @@ example (a b : Prop) (ha : a) (hab : a → b) : b := by
       let goal ← getMainGoal
       let lctx ← getLCtx
       -- find appropriate free variables
-      let some ehab := lctx.findFromUserName? `hab | throwError "not found"
-      let some eha := lctx.findFromUserName? `ha | throwError "not found"
+      let some ehab := lctx.findFromUserName? `hab | throwError "hab not found"
+      let some eha := lctx.findFromUserName? `ha | throwError "ha not found"
       let e : Expr := (.app -- build the term "hab ha"
-        (mkFVar ehab.fvarId)
-        (mkFVar eha.fvarId)
+        (.fvar ehab.fvarId)
+        (.fvar eha.fvarId)
       )
       let t ← inferType e -- t = "b", e = "hab hb"
       -- goal: ctx |- mainGoal
@@ -505,9 +491,7 @@ example (a b : Prop) (ha : a) (hab : a → b) : b := by
       let (_, goal3) ← goal2.intro `hb
       -- goal3: ctx, t |- mainGoal
       replaceMainGoal [goal3]
-  exact hb -- look at the tactic state before closing the goal ;-)
-
-end Chapter4TacticCode
+  exact hb
 
 /-
 ## (5) How to declare syntax for a new tactic
@@ -533,13 +517,13 @@ Another nice resource of what could be a problem when you get stuck
 on a mysterious metaprogramming problem:
 https://github.com/leanprover-community/mathlib4/wiki/Metaprogramming-gotchas
 
-But also, just be curious -- ctrl-click on the functions we are using
+But also, just be curious - ctrl-click on the functions we are using
 to see what they are doing.
 
-You can also ctrl-click on a monad, such as
-TacticM or MetaM (and others you will get into such as TermElabM),
-and you will see the extra states it has
-(as Context & State), as well as the monad below.
-There states can be a bit scary but all the information Lean
+You can also ctrl-click on a monad, such as `TacticM` or `MetaM`
+(and others you may run into such as `TermElabM`, `CoreM`, `IO`, `MacroM`, `DelabM`),
+and you will see the extra states it has (as `Context` & `State`), as well as
+what other monad it extends, if any.
+These states can be a bit scary but all the information Lean
 has to its disposal must be somewhere in them...
 -/
